NumLean/Interfaces/UntypedIndex.lean
@@ -1,0 +1,31 @@
+import Mathlib.Logic.Equiv.Defs
+import Mathlib.Logic.Equiv.Fin.Basic
+
+namespace NumLean
+
+class UntypedIndex (idx : Type u) (idx' : outParam (Type v)) (dom : outParam (idx' → Prop)) where
+  equiv : idx ≃ { i : idx' // dom i }
+
+open UntypedIndex
+
+variable [UntypedIndex I I' dom]
+
+@[simp]
+theorem dom_equiv (i : I) : dom (equiv i) := (equiv i).2
+
+instance : UntypedIndex (Fin n) Nat (· < n) where
+  equiv := {
+    toFun x := ⟨x.1, x.2⟩
+    invFun x := ⟨x.1, x.2⟩
+    left_inv := by intro; rfl
+    right_inv := by intro; rfl
+  }
+
+instance [UntypedIndex I I' idom] [UntypedIndex J J' jdom] :
+    UntypedIndex (I × J) (I' × J') (fun ⟨i,j⟩ => idom i ∧ jdom j) where
+  equiv := {
+    toFun := fun ⟨i,j⟩ => ⟨(equiv i, equiv j), by simp⟩
+    invFun := fun ⟨(i,j),h⟩ => (equiv.symm ⟨i, by simp_all⟩, equiv.symm ⟨j, by simp_all⟩)
+    left_inv := by intro; simp
+    right_inv := by intro; simp
+  }
