NumLean/Meta.lean
@@ -1,3 +1,2 @@
-import NumLean.Meta.CCompiler
 import NumLean.Meta.ForAll
 import NumLean.Meta.RewriteBy
