NumLean/Meta/CCompiler.lean
@@ -1,1 +1,0 @@
-import NumLean.Meta.CCompiler.Command
