NumLean/Widget/Visualize/Command.lean
@@ -1,0 +1,50 @@
+import Lean.Elab.Command
+import Qq
+import NumLean.Widget.Visualize.Visualizers
+
+namespace NumLean
+namespace Widget
+
+open Lean Server Elab Command ProofWidgets
+
+/-- Generic visualization command.
+
+Examples:
+```lean
+#visualize hp(•,(•,•))
+#visualize #[hp(•,•), hp(•,(•,•))]
+#visualize (hp(•,•), ({ offset := 0, stride := h((1 : Int), (4 : Int)) } :
+  Cute.Layout h((4 : Nat), (8 : Nat)) Int))
+```
+-/
+syntax (name := visualizeCmd) "#visualize" term : command
+
+open Meta Elab Term Qq in
+@[command_elab visualizeCmd]
+def elabVisualize : CommandElab := fun stx => do
+  match stx with
+  | `(#visualize $x:term) => do
+      let (rpc, js) ← liftTermElabM <| do
+        let xExpr ← instantiateMVars (← elabTermAndSynthesize x none)
+        let xTy ← instantiateMVars (← inferType xExpr)
+        let visTy ← mkFreshTypeMVar
+        let visInstType := mkAppN (← mkConstWithFreshMVarLevels ``Visualizable) #[xTy, visTy]
+        let visInst ← synthInstance visInstType
+        let visTy ← instantiateMVars visTy
+        let rendererInstType := mkApp (← mkConstWithFreshMVarLevels ``Visualizer) visTy
+        let rendererInst ← synthInstance rendererInstType
+        let rpcExpr ← instantiateMVars
+          (← mkAppOptM ``Visualizable.toRpc #[xTy, visTy, visInst, rendererInst, xExpr])
+        let jsExpr ← instantiateMVars
+          (← mkAppOptM ``Visualizable.javascriptFor #[xTy, visTy, visInst, rendererInst, xExpr])
+        let rpc ← unsafe evalExpr (StateM RpcObjectStore Json) q(StateM RpcObjectStore Json) rpcExpr
+        let js ← unsafe evalExpr String q(String) jsExpr
+        pure (rpc, js)
+      liftCoreM <| Lean.Widget.savePanelWidgetInfo
+        (hash js)
+        rpc
+        stx
+  | _ => throwUnsupportedSyntax
+
+end Widget
+end NumLean
